src/tls/KeySchedule.fst
@@ -8,7 +8,6 @@ open FStar.Heap
 open FStar.HyperHeap
 open FStar.HyperStack
 open FStar.Seq
-open FStar.SeqProperties
 open FStar.Set  
 
 open Platform.Bytes
