src/tls/StreamAE.fst
@@ -8,7 +8,7 @@ open FStar.Heap
 open FStar.HyperHeap
 open FStar.HyperStack
 open FStar.Seq
-open FStar.SeqProperties // for e.g. found
+ // for e.g. found
 open FStar.Monotonic.RRef
 open FStar.Monotonic.Seq
 
