src/tls/artifact/StatefulLHAE.fst
@@ -9,7 +9,7 @@ module StatefulLHAE
 open FStar.Heap
 open FStar.HyperHeap
 open FStar.Seq
-open FStar.SeqProperties // for e.g. found
+ // for e.g. found
 
 open Platform.Bytes
 
