src/tls/artifact/TLSConstants.fst
@@ -14,7 +14,7 @@ open Platform.Bytes
 open Platform.Error
 open TLSError
 open CoreCrypto
-open FStar.SeqProperties
+open FStar.Seq
 
 (* Type representations for TLS negotiated values *)
 type protocolVersion =
@@ -807,7 +807,7 @@ val lemma_vlbytes_inj : i:nat
                    (ensures (b=b'))
 let lemma_vlbytes_inj i b b' =
   let l = bytes_of_int i (length b) in
-  SeqProperties.lemma_append_inj l b l b'
+  Seq.lemma_append_inj l b l b'
 
 #set-options "--max_ifuel 1 --initial_ifuel 1 --max_fuel 0 --initial_fuel 0"   //need to reason about length
 val vlsplit: lSize:nat{lSize <= 4}
